theories/logrel/fundamental_prim.v
@@ -1,0 +1,23 @@
+From iris.proofmode Require Import tactics.
+From machine_program_logic.program_logic Require Import weakestpre.
+From HypVeri.lang Require Import lang trans_extra.
+From HypVeri.algebra Require Import base pagetable mem trans.
+From HypVeri.rules Require Import rules_base mov yield ldr halt fail add sub mult cmp br bne str run.
+From HypVeri.logrel Require Import logrel_prim.
+(* From HypVeri.logrel Require Import ftlr_nop ftlr_run ftlr_yield ftlr_share ftlr_retrieve ftlr_relinquish ftlr_reclaim ftlr_donate ftlr_lend *)
+(*   ftlr_msg_send ftlr_msg_wait ftlr_msg_poll ftlr_invalid_hvc. *)
+From HypVeri Require Import proofmode.
+Import uPred.
+
+Section fundamental_prim.
+  Context `{hypconst:HypervisorConstants}.
+  Context `{hypparams:!HypervisorParameters}.
+  Context `{vmG: !gen_VMG Σ}.
+
+  Lemma ftlr_p:
+  ∀ p_tx p_rx ps_acc trans, interp_access_prim p_tx p_rx ps_acc trans ⊢ interp_execute V0.
+  Proof.
+    rewrite /interp_access_prim /=.
+  Admitted.
+
+End fundamental_prim.
