theories/logrel/logrel_prim.v
@@ -1,0 +1,60 @@
+From iris.proofmode Require Import tactics.
+From machine_program_logic.program_logic Require Import weakestpre.
+From HypVeri.lang Require Import lang.
+From HypVeri.algebra Require Import base base_extra mem mailbox trans.
+From HypVeri.logrel Require Export logrel logrel_extra.
+
+Section logrel_prim.
+
+  Context `{hypconst:HypervisorConstants}.
+  Context `{hypparams:!HypervisorParameters}.
+  Context `{vmG: !gen_VMG Σ}.
+
+  Definition trans_rel_primary (i:VMID) (trans trans': gmap Word transaction): Prop :=
+   map_Forall (λ h tran,
+          ((tran.1.1.1.1 ≠ i ∧ tran.1.1.1.2 ≠ i) -> ∃ tran', trans' !! h = Some tran' ∧ tran = tran') ∧
+          ((tran.1.1.1.1 = i ∧ tran.2 = true) -> ∃ tran', trans' !! h = Some tran' ∧ tran = tran') ∧
+          ((tran.1.1.1.2= i ∧ tran.1.2 ≠ Donation) -> ∃ tran', trans' !! h = Some tran' ∧ tran.1 = tran'.1)
+     ) trans.
+
+  Definition transaction_pagetable_entries_transferred_all (trans: gmap Addr transaction) : iProp Σ:=
+    big_sepFM trans (λ kv, kv.2.1.2 = Donation) (λ k v, k -{1/4}>t v.1 ∗ pgt_1_4 v.1.1.2 v.1.1.1.1 true)%I.
+
+  Definition retrievable_transaction_transferred_all(trans: gmap Addr transaction) : iProp Σ:=
+    (big_sepFM trans (λ kv, True) (λ k v, k -{1/2}>re v.2 )%I) ∗
+    (big_sepFM trans (λ kv, kv.2.2 = false) (λ k v, k -{1/4}>t v.1 ∗ k -{1/2}>re v.2)%I).
+
+  Definition transaction_pagetable_entries_transferred_except (i: VMID) (trans: gmap Addr transaction) : iProp Σ:=
+    big_sepFM trans (λ kv, kv.2.1.2 = Donation ∧ ¬(kv.2.1.1.1.2 = i ∨ kv.2.1.1.1.1 = i)) (λ k v, k -{1/4}>t v.1 ∗ pgt_1_4 v.1.1.2 v.1.1.1.1 true)%I.
+
+  Definition retrievable_transaction_transferred_except (i: VMID) (trans: gmap Addr transaction) : iProp Σ:=
+    (big_sepFM trans (λ kv, ¬(kv.2.1.1.1.2 = i ∨ kv.2.1.1.1.1 = i)) (λ k v, k -{1/2}>re v.2 )%I) ∗
+    (big_sepFM trans (λ kv, ¬(kv.2.1.1.1.2 = i ∨ kv.2.1.1.1.1 = i) ∧ kv.2.2 = false) (λ k v, k -{1/4}>t v.1 ∗ k -{1/2}>re v.2)%I).
+
+  Definition transferred_memory_pages_all (trans : gmap Word transaction) :=
+    pages_in_trans (filter (λ kv, ¬(kv.2.2 = true ∧ kv.2.1.2 = Lending)) trans).
+
+  Program Definition interp_access_prim p_tx p_rx ps_acc trans: iPropO Σ:=
+    (
+      let ps_macc_trans := (transferred_memory_pages_all trans) in
+      let ps_oea := ps_acc ∖ {[p_rx;p_tx]} ∖ (currently_accessible_in_trans_memory_pages V0 trans) in
+      (∃ regs, ⌜is_total_gmap regs⌝ ∗ [∗ map] r ↦ w ∈ regs, r @@ V0 ->r w) ∗
+      (tx_page V0 p_tx ∗ ∃ mem_tx, memory_page p_tx mem_tx) ∗
+      V0 -@A> ps_acc ∗
+      ⌜{[p_tx;p_rx]} ⊆ ps_acc⌝ ∗ ⌜currently_accessible_in_trans_memory_pages V0 trans ⊆ ps_acc ∖ {[p_tx;p_rx]}⌝ ∗
+      pagetable_entries_excl_owned V0 ps_oea ∗
+      transaction_pagetable_entries_owned V0 trans ∗
+      retrieved_transaction_owned V0 trans ∗
+      (∃ mem_oea, memory_pages (ps_oea ∪ (retrieved_lending_memory_pages V0 trans)) mem_oea) ∗
+      VMProp V0 True 1%Qp ∗
+      (* transferred *)
+      (∃ rx_state, RX_state@ V0 := rx_state) ∗ (rx_page V0 p_rx) ∗ (∃ mem_rx, memory_page p_rx mem_rx) ∗
+      transaction_hpool_global_transferred trans ∗
+      transaction_pagetable_entries_transferred_all trans ∗
+      retrievable_transaction_transferred_all trans ∗
+      (∃ mem_trans, memory_pages ps_macc_trans mem_trans) ∗
+      rx_pages (list_to_set (list_of_vmids) ∖ {[V0]}) ∗
+      [∗ set] i ∈ list_to_set (list_of_vmids) ∖ {[V0]}, VMProp (i:VMID) (vmprop_unknown i p_tx p_rx) (1/2)%Qp
+    )%I.
+
+End logrel_prim.
