theories/logrel/logrel_prim_extra.v
@@ -1,0 +1,56 @@
+From iris.proofmode Require Import tactics.
+From machine_program_logic.program_logic Require Import weakestpre.
+From HypVeri.lang Require Import lang.
+From HypVeri.algebra Require Import base base_extra mem pagetable trans.
+From HypVeri.logrel Require Import logrel_prim.
+From HypVeri Require Import proofmode.
+From stdpp Require fin_map_dom.
+Import uPred.
+
+Section logrel_prim_extra.
+  Context `{hypconst:HypervisorConstants}.
+  Context `{hypparams:!HypervisorParameters}.
+  Context `{vmG: !gen_VMG Σ}.
+
+  (* Lemmas about relationships between transferred_all, transferred, and transferred_except *)
+  Lemma transaction_pagetable_entries_transferred_split i trans:
+    transaction_pagetable_entries_transferred_all trans ⊣⊢ transaction_pagetable_entries_transferred i trans ∗
+                                                 transaction_pagetable_entries_transferred_except i trans.
+  Proof. iApply (big_sepFM_split_decide). Qed.
+
+  Lemma retrievable_transaction_transferred_split i trans:
+   retrievable_transaction_transferred_all trans ⊣⊢ retrievable_transaction_transferred i trans ∗
+                                                 retrievable_transaction_transferred_except i trans.
+  Proof.
+    rewrite /retrievable_transaction_transferred /retrievable_transaction_transferred_all /retrievable_transaction_transferred_except.
+    iSplit.
+    iIntros "(H1 & H2)".
+    iDestruct (big_sepFM_split_decide (Q:= (λ kv, kv.2.1.1.1.2 = i ∨ kv.2.1.1.1.1 = i)) with "H1") as "[H11 H12]".
+    rewrite (big_sepFM_iff (Q:= (λ kv, kv.2.1.1.1.2 = i ∨ kv.2.1.1.1.1 = i))). iFrame "H11".
+    rewrite (big_sepFM_iff (Q:= (λ kv, ¬ (kv.2.1.1.1.2 = i ∨ kv.2.1.1.1.1 = i)))). iFrame "H12".
+    iDestruct (big_sepFM_split_decide (Q:= (λ kv, kv.2.1.1.1.1 = i ∨ kv.2.1.1.1.2 = i)) with "H2") as "[H21 H22]".
+    iSplitL "H21".
+    iApply (big_sepFM_iff with "H21"). intros. split;intros [? ?];auto.
+    iApply (big_sepFM_iff with "H22"). intros. split;intros [? ?];split;auto. intro Hor;apply H;destruct Hor;eauto.
+    intro Hor;apply H0;destruct Hor;eauto.
+    intros. split;intros H;eauto. destruct H;done.
+    intros. split;intros H;eauto. destruct H;done.
+    iIntros "([H11 H12] & [H21 H22])".
+    iSplitL "H11 H21".
+    iApply (big_sepFM_split_decide (Q:= (λ kv, kv.2.1.1.1.2 = i ∨ kv.2.1.1.1.1 = i))).
+    rewrite (big_sepFM_iff (Q:= (λ kv, kv.2.1.1.1.2 = i ∨ kv.2.1.1.1.1 = i))). iFrame "H11".
+    rewrite (big_sepFM_iff (Q:= (λ kv, ¬ (kv.2.1.1.1.2 = i ∨ kv.2.1.1.1.1 = i)))). iFrame "H21".
+    intros. split;intros H;eauto. destruct H;done.
+    intros. split;intros H;eauto. destruct H;done.
+    iApply (big_sepFM_split_decide (Q:= (λ kv, kv.2.1.1.1.1 = i ∨ kv.2.1.1.1.2 = i))).
+    iSplitL "H12".
+    iApply big_sepFM_iff. 2: iFrame "H12".
+    intros. split;intros H;eauto. destruct H;auto. destruct H;split;auto.
+    iApply big_sepFM_iff. 2: iFrame "H22".
+    intros. split;intros H;eauto. destruct H as [? H];split;auto.
+    intro. apply H. destruct H1;auto.
+    destruct H as [? H];split;auto.
+    intro. apply H0. destruct H1;auto.
+  Qed.
+
+End logrel_prim_extra.
